Add old ModelCount code

lean4/ModelCount/ModelCount/Iteg.lean
@@ -3,7 +3,7 @@ import ModelCount.Lib
 /- itegs-/
 
 inductive IteElt
-  | Tr                : IteElt 
+  | Tr                : IteElt
   | Fls               : IteElt
   | Var (i : Nat)     : IteElt
   | Ite (c t f : Nat) : IteElt
@@ -20,22 +20,24 @@ def IteEltBounded : IteElt → Nat → Prop
   | Var i,     _ => True
   | Ite c t f, b => t < b ∧ f < b
 
--- No need to bound i, since the default value of an `IteElt` is `Tr` 
+-- No need to bound i, since the default value of an `IteElt` is `Tr`
 def Iteg := { I : Array IteElt // ∀ i, IteEltBounded I[i] i }
 
 -- coerce to an array
 instance itegCoe (n : Nat) : CoeHead Iteg (Array IteElt) where coe v := v.val
 
--- TODO: a hack to fix an annoying dependcy; find a better way
+-- TODO: a hack to fix an annoying dependency; find a better way
 theorem match_aux (i : IteElt) (a b : α) (c : Nat → α) (d : Nat → Nat → Nat → α) :
     (match h:i with | Tr => a | Fls => b | Var j => c j | Ite c t f => d c t f) =
-      (match i with | Tr => a | Fls => b | Var j => c j | Ite c t f => d c t f) := 
+      (match i with | Tr => a | Fls => b | Var j => c j | Ite c t f => d c t f) :=
 by cases i <;> rfl
 
 
 /- semantics: the `eval` function -/
 
 def Assignment : Type := Nat → Bool
+
+noncomputable instance : DecidableEq α := fun a b => Classical.propDecidable _
 
 namespace Iteg
 
@@ -44,21 +46,21 @@ def evalF (I : Iteg) (v : Assignment) (m : Nat) (eval_rec : (∀ i, i < m → Bo
     | Tr            => true
     | Fls           => false
     | Var k         => v k
-    | Ite c t f     => 
-        have bdd : IteEltBounded (Ite c t f) m by { rw ←h; apply I.property }
+    | Ite c t f     =>
+        have bdd : IteEltBounded (Ite c t f) m :=  by { rw [←h]; apply I.property }
         cond (v c) (eval_rec _ bdd.1) (eval_rec _ bdd.2)
 
 
 /-- `I.eval v j` evaluated line `j` of iteg `I` with assignment `v` -/
-noncomputable def eval (I : Iteg) (v : Assignment) : Nat → Bool := 
+noncomputable def eval (I : Iteg) (v : Assignment) : Nat → Bool :=
 WellFounded.fix Nat.ltWf (evalF I v)
 
-theorem eval_eq (I : Iteg) (v : Assignment) (j : Nat) : 
-  eval I v j = match I.val[j] with 
+theorem eval_eq (I : Iteg) (v : Assignment) (j : Nat) :
+  eval I v j = match I.val[j] with
                  | Tr        => true
                  | Fls       => false
-                 | Var k     => v k 
-                 | Ite c t f => cond (v c) (eval I v t) (eval I v f) := 
+                 | Var k     => v k
+                 | Ite c t f => cond (v c) (eval I v t) (eval I v f) :=
 by
   apply Eq.trans $ WellFounded.fixEq Nat.ltWf (evalF I v) j
   apply Eq.trans _ (match_aux _ _ _ _ _); rfl
@@ -75,40 +77,40 @@ by
 end Iteg
 
 namespace Iteg
-open Finset
+open List
 
 /- the `vars` function -/
 
-def varsF (I : Iteg) (m : Nat) (vars_rec : (∀ i, i < m → Finset Nat)) : Finset Nat :=
+def varsF (I : Iteg) (m : Nat) (vars_rec : (∀ i, i < m → List Nat)) : List Nat :=
   match h:I.val[m] with
     | Tr            => ∅
     | Fls           => ∅
-    | Var j         => singleton j
+    | Var j         => [j]
     | Ite c t f     =>
-        have bdd : IteEltBounded (Ite c t f) m by { rw ←h; apply I.property }
-        singleton c ∪ (vars_rec _ bdd.1) ∪ (vars_rec _ bdd.2)
+        have bdd : IteEltBounded (Ite c t f) m := by { rw [←h]; apply I.property }
+        insert c ((vars_rec _ bdd.1).union (vars_rec _ bdd.2))
 
-/-- `I.vars j` returns the `Finset` of variables that line `j` iteg `I` depends on. -/
-noncomputable def vars (I : Iteg) : Nat → Finset Nat := WellFounded.fix Nat.ltWf (varsF I)
+/-- `I.vars j` returns the list of variables that line `j` iteg `I` depends on. -/
+noncomputable def vars (I : Iteg) : Nat → List Nat := WellFounded.fix Nat.ltWf (varsF I)
 
-theorem vars_eq (I : Iteg) (j : Nat) : 
-  vars I j = match I.val[j] with 
+theorem vars_eq (I : Iteg) (j : Nat) :
+  vars I j = match I.val[j] with
                | Tr        => ∅
                | Fls       => ∅
-               | Var k     => singleton k
-               | Ite c t f => singleton c ∪ vars I t ∪ vars I f := 
+               | Var k     => [k]
+               | Ite c t f => insert c ((vars I t).union (vars I f)) :=
 by
   apply Eq.trans $ WellFounded.fixEq Nat.ltWf (varsF I) j
   apply Eq.trans _ (match_aux _ _ _ _ _); rfl
 
 @[simp] theorem vars_Tr {I : Iteg} {j : Nat} (h : I.val[j] = Tr) :
-  I.vars j = (∅ : Finset Nat) := by rw [vars_eq, h]
+  I.vars j = (∅ : List Nat) := by rw [vars_eq, h]
 @[simp] theorem var_Fls {I : Iteg} {j : Nat} (h : I.val[j] = Fls) :
-  I.vars j = (∅ : Finset Nat) := by rw [vars_eq, h]
+  I.vars j = (∅ : List Nat) := by rw [vars_eq, h]
 @[simp] theorem vars_Var {I : Iteg} {j k : Nat} (h : I.val[j] = Var k) :
-  I.vars j = singleton k := by rw [vars_eq, h]
+  I.vars j = [k] := by rw [vars_eq, h]
 @[simp] theorem vars_Ite {I : Iteg} {j c t f : Nat} (h : I.val[j] = Ite c t f) :
-  I.vars j = singleton c ∪ I.vars t ∪ I.vars f := by rw [vars_eq, h]
+  I.vars j = insert c ((I.vars t).union (I.vars f)) := by rw [vars_eq, h]
 
 
 /- the `count` function -/
@@ -119,21 +121,21 @@ def countF (I : Iteg) (numVars : Nat) (m : Nat) (count_rec : ∀ i, i < m → Na
     | Fls           => 0
     | Var j         => 2 ^ (numVars - 1)
     | Ite c t f     =>
-        have bdd : IteEltBounded (Ite c t f) m by { rw ←h; apply I.property }
+        have bdd : IteEltBounded (Ite c t f) m := by { rw [←h]; apply I.property }
         (count_rec _ bdd.1 + count_rec _ bdd.2) / 2
 
-/-- 
+/--
 `I.count I j` counts the number of models of line `j` of iteg `I`, assuming `numVars` variables in total.
 -/
-noncomputable def count (I : Iteg) (numVars : Nat) : Nat → Nat := 
+noncomputable def count (I : Iteg) (numVars : Nat) : Nat → Nat :=
 WellFounded.fix Nat.ltWf (countF I numVars)
 
-theorem count_eq (I : Iteg) (numVars : Nat) (j : Nat) : 
-  count I numVars j = match I.val[j] with 
-                        | Tr        => 2 ^ numVars
+theorem count_eq (I : Iteg) (numVars : Nat) (j : Nat) :
+  count I numVars j = match I.val[j] with
+                        | Tr        => 2^ numVars
                         | Fls       => 0
                         | Var k     => 2 ^ (numVars - 1)
-                        | Ite c t f => (count I numVars t + count I numVars f) / 2 := 
+                        | Ite c t f => (count I numVars t + count I numVars f) / 2 :=
 by
   apply Eq.trans $ WellFounded.fixEq Nat.ltWf (countF I numVars) j
   apply Eq.trans _ (match_aux _ _ _ _ _); rfl
@@ -150,70 +152,215 @@ by
 
 /- free itegs -/
 
-def free (I : Iteg) : Prop := 
+def free (I : Iteg) : Prop :=
 ∀ j, match I.val[j] with
        | Tr => True
        | Fls => True
        | Var k => True
-       | Ite c t f => c ∉ I.vars t ∧ c ∉ I.vars f
+       | Ite c t f => (c ∉ I.vars t) ∧ (c ∉ I.vars f)
 
 
 /- counting models assignments -/
 
-def defined_on (v : Assignment) (s : Finset Nat) := ∀ n, ¬ n ∈ s → v n = false
+def defined_on (v : Assignment) (s : List Nat) := ∀ n, ¬ n ∈ s → v n = false
 
-theorem finite_defined_on (s : Finset Nat) : Set.finite (fun v : Assignment => defined_on v s) :=
-sorry
+def update (n : Nat) (b : Bool) (v : Assignment) := fun i => if i = n then b else v i
 
-def models (s : Finset Nat) : Finset Assignment := ⟨_, finite_defined_on s⟩
+theorem update_self (n : Nat) (b : Bool) (v : Assignment) :
+  update n b v n = b := by simp [update]
 
-@[simp] theorem card_models (s : Finset Nat) : card (models s) = 2 ^ card s :=
-sorry
+theorem update_pos {n : Nat} {i : Nat} (h : i = n) (b : Bool) (v : Assignment) :
+  update n b v i = b := by simp [update, h]
 
+theorem update_neg {n : Nat} {i : Nat} (h : i ≠ n) (b : Bool) (v : Assignment) :
+  update n b v i = v i := by simp [update, h]
+
+theorem update_update (n : Nat) (b₁ b₂ : Bool) (v : Assignment) :
+    update n b₁ (update n b₂ v) = update n b₁ v := by
+  apply funext
+  intro n'
+  cases Decidable.em (n' = n) with
+  | inl h => rw [←h, update_self, update_self]
+  | inr h => rw [update_neg h, update_neg h, update_neg h]
+
+theorem update_same (n : Nat) (v : Assignment) : update n (v n) v = v := by
+  apply funext
+  intro n'
+  cases Decidable.em (n' = n) with
+  | inl h => rw [←h, update_self]
+  | inr h => rw [update_neg h]
+
+noncomputable def models : List Nat → List Assignment
+  | [] => [fun n => false]
+  | (n :: ns) => if n ∈ ns then models ns else (models ns).union ((models ns).map (update n true))
+
+theorem mem_models (s : List Nat) (v : Assignment) : v ∈ models s ↔ defined_on v s := by
+  induction s generalizing v with
+  | nil =>
+    simp [models, defined_on]
+    split
+      intros h n; rw [h]
+    apply funext
+  | cons n ns ih =>
+    simp [models, defined_on]
+    cases Decidable.em (n ∈ ns) with
+    | inl h =>
+      simp [h, ih, defined_on]
+      split; focus
+        intros h' n' hn'
+        apply h'; intro h''; exact hn' (Or.inr h'')
+      intros h' n' hn'
+      apply h'
+      intros h''
+      have : n' = n := Or.resolve_right h'' hn'
+      rw [this] at hn'
+      exact hn' h
+    | inr h =>
+      simp [h, ih, defined_on, mem_map]
+      split; focus
+        intros h' n' hn'
+        match h' with
+        | Or.inl h'' =>
+          apply h''
+          intro h₃
+          exact hn' (Or.inr h₃)
+        | Or.inr ⟨v', h₃, h₄⟩ =>
+          rw [not_or] at hn'
+          have : v n' = v' n' := by rw [h₄, update_neg hn'.1]
+          rw [this]
+          apply h₃ _ hn'.2
+      intros h'
+      cases Bool.eq_true_or_eq_false (v n) with
+      | inl h'' =>
+        apply Or.inr
+        apply Exists.intro (update n false v)
+        split; focus
+          intro n' hn'
+          cases Decidable.em (n' = n) with
+          | inl h₃ => rw [h₃, update_self]
+          | inr h₃ => rw [update_neg h₃]; apply h'; rw [not_or]; apply ⟨h₃, hn'⟩
+        rw [update_update, ←h'', update_same]
+      | inr h'' =>
+        apply Or.inl
+        intro n' hn'
+        cases Decidable.em (n' = n) with
+        | inl h₃ => rw [h₃, h'']
+        | inr h₃ => apply h'; rw [not_or]; exact ⟨h₃, hn'⟩
+
+theorem inj_on_update {s : List Nat} {n : Nat} (h : n ∉ s) (b : Bool) :
+    inj_on (update n b) (models s) := by
+  intros v₁ v₂
+  rw [mem_models, mem_models]
+  intros h1 h2 h3
+  apply funext; intro n'
+  cases Decidable.em (n' = n) with
+  | inl h4 => rw [h4, h1 _ h, h2 _ h]
+  | inr h4 => rw [←update_neg h4 b v₁, h3, update_neg h4]
+
+@[simp] theorem card_models (s : List Nat) : card (models s) = 2 ^ card s := by
+  induction s with
+  | nil => rfl
+  | cons n ns ih =>
+    simp [models, card]
+    cases Decidable.em (n ∈ ns) with
+    | inl h => simp [h, ih]
+    | inr h =>
+      simp [h, Nat.pow_succ]
+      have dsj : disjoint (models ns) (map (update n true) (models ns)) := by
+        intros v hv h'v
+        rw [mem_models] at hv
+        rw [mem_map] at h'v
+        match h'v with
+        | ⟨v', hv', h'v'⟩ =>
+          have : false = true := by rw [←hv _ h, h'v', update_self]
+          contradiction
+      have inj : inj_on (update n true) (models ns) := inj_on_update h _
+      rw [card_union_disjoint dsj, card_map_eq_of_inj_on inj, ih, Nat.mul_two]
 
 /- auxiliary lemmas -/
 
-theorem card_models_Var {s : Finset Nat} {k : Nat} (h : k ∈ s) : 
-  card {v ∈ models s | v k = True} = 2 ^ (card s - 1) :=
-sorry
+theorem card_models_Var {s : List Nat} {k : Nat} (h : k ∈ s) :
+    card ((models s).filter (λ v => v k)) = 2 ^ (card s - 1) := by
+  have : ((models s).filter (λ v => v k)).equiv ((models (s.remove k)).map (update k true)) := by
+    intro v
+    rw [mem_filter, mem_map, mem_models]
+    split; focus
+      intro ⟨h1, h2⟩
+      refine ⟨update k false v, ?_⟩
+      split; focus
+        rw [mem_models]
+        intros j hj
+        rw [mem_remove_iff, Classical.not_and, Classical.dne] at hj
+        cases Decidable.em (j = k) with
+        | inl h3 => rw [update_pos h3]
+        | inr h3 => rw [update_neg h3, h1 _ (Or.resolve_right hj h3)]
+      rw [update_update, ←h2, update_same]
+    intro ⟨v', h1v', h2v'⟩
+    rw [mem_models] at h1v'
+    simp [h2v', update_self]
+    intros j hj
+    have : j ≠ k := by intro h4; apply hj; rw [h4]; exact h
+    rw [update_neg this]
+    apply h1v'
+    rw [mem_remove_iff, Classical.not_and]; simp [hj]
+  rw [card_eq_of_equiv this, card_map_eq_of_inj_on (inj_on_update (not_mem_remove _ _) _),
+    card_models, card_remove_of_mem' h]
+
+theorem aux1 {t : Nat} {I : Iteg} {s : List Nat} (h₀ : c ∈ s) (h₁ : ¬c ∈ vars I t) :
+  card ((models s).filter (fun (v : Assignment) => eval I v t)) =
+    2 * card ((models s).filter (fun (v : Assignment) => v c && eval I v t)) := sorry
+
+theorem aux2 {f : Nat} {I : Iteg} {s : List Nat} (h₀ : c ∈ s) (h₁ : ¬c ∈ vars I f) :
+  card ((models s).filter (fun (v : Assignment) => eval I v f)) =
+    2 * card ((models s).filter (fun (v : Assignment) => !v c && eval I v f)) := sorry
 
 /- this is the main combinatorial lemma behind the counting algorithm -/
-theorem card_models_Ite {I : Iteg} {s : Finset Nat} {c : Nat} 
-    (h₀ : c ∈ s) (h₁ : c ∉ I.vars t) (h₂ : c ∉ I.vars f) : 
-  card {v ∈ models s | cond (v c) (eval I v t) (eval I v f) = true} =
-    (card {v ∈ models s | eval I v t = true} + card {v ∈ models s | eval I v f = true}) / 2 := 
-sorry
+theorem card_models_Ite {I : Iteg} {s : List Nat} {c : Nat}
+    (h₀ : c ∈ s) (h₁ : c ∉ I.vars t) (h₂ : c ∉ I.vars f) :
+  card ((models s).filter (λ v => cond (v c) (eval I v t) (eval I v f))) =
+    (card ((models s).filter (λ v => eval I v t)) +
+      card ((models s).filter (λ v => eval I v f))) / 2 := by
+  apply Eq.symm
+  apply Nat.div_eq_of_eq_mul_right; exact Nat.zero_lt_succ _
+  have : ((models s).filter (λ v => cond (v c) (eval I v t) (eval I v f))).equiv
+      (((models s).filter (λ v => v c && (eval I v t))).union
+       ((models s).filter (λ v => !(v c) &&(eval I v f)))) := by
+    intro v
+    simp [mem_filter]; cases (v c) <;> simp
+  rw [card_eq_of_equiv this, card_union_disjoint, Nat.mul_add, aux1 h₀ h₁, aux2 h₀ h₂]
+  intro v
+  simp [mem_filter]; cases (v c) <;> simp
 
 
 /- the main theorem -/
 
-theorem card_models_Iteg (I : Iteg) (v : Assignment) (s : Finset Nat) (Ifree : free I): 
-   ∀ j, I.vars j ⊆ s →  card {v ∈ models s | I.eval v j = true} = I.count (card s) j := 
+theorem card_models_Iteg (I : Iteg) (Ifree : free I) (v : Assignment) (s : List Nat) :
+   ∀ j, I.vars j ⊆ s →  card ((models s).filter (λ v => I.eval v j)) = I.count (card s) j :=
 by
   intro j
   induction j using Nat.CompleteInductionOn with
     | ind j ih =>
-      rw count_eq
+      rw [count_eq]
       cases h:I.val[j] with
       | Tr        => simp [h]
       | Fls       => simp [h]
       | Var k     =>
           simp [vars_Var h, eval_Var h]
           apply card_models_Var
-      | Ite c t f => 
-          have bdd : IteEltBounded (Ite c t f) j by { rw ←h; apply I.property }
-          have _ := Ifree j
-          rw h at this
-          have free: c ∉ I.vars t ∧ c ∉ I.vars f from this
+      | Ite c t f =>
+          have bdd : IteEltBounded (Ite c t f) j := by { rw [←h]; apply I.property }
+          have := Ifree j
+          rw [h] at this
+          have free: (c ∉ I.vars t) ∧ (c ∉ I.vars f) := this
           simp [vars_Ite h, eval_Ite h]
           intro h'
-          have h₀ : c ∈ s from singleton_subset.mp (subset_trans (subset_union_left _ _) h')
-          have h₁ : vars I t ⊆ s from subset_trans (subset_union_left _ _) 
-                                        (subset_trans (subset_union_right _ _) h')
-          have h₂ : vars I f ⊆ s from subset_trans (subset_union_right _ _) 
-                                        (subset_trans (subset_union_right _ _) h')
-          have h₃ : card {v ∈ models s | I.eval v t = true} = count I (card s) t from ih _ bdd.1 h₁
-          have h₄ : card {v ∈ models s | I.eval v f = true} = count I (card s) f from ih _ bdd.2 h₂
+          have h₀ : c ∈ s := h' (mem_insert_self _ _)
+          have h₁ : vars I t ⊆ s := subset_trans (subset_union_left _ _)
+                                        (subset_trans (subset_insert _ _) h')
+          have h₂ : vars I f ⊆ s := subset_trans (subset_union_right _ _)
+                                        (subset_trans (subset_insert _ _) h')
+          have h₃ : card ((models s).filter (λ v => I.eval v t)) = count I (card s) t := ih _ bdd.1 h₁
+          have h₄ : card ((models s).filter (λ v => I.eval v f)) = count I (card s) f := ih _ bdd.2 h₂
           rw [←h₃, ←h₄]
           apply card_models_Ite h₀ free.1 free.2
 
@@ -227,7 +374,7 @@ def countModelsStep (I : Array IteElt) (numVars : Nat) (i : Nat) (O : Array Nat)
             | Var k      => 2^ (numVars - 1)
             | Ite c t f  => (O[t] + O[f]) / 2
 
-def countModels (I : Array IteElt) (numVars : Nat) : Array Nat := do 
+def countModels (I : Array IteElt) (numVars : Nat) : Array Nat := do
   let mut O : Array Nat := #[]
   for i in [:I.size] do O := countModelsStep I numVars i O
   return O
@@ -240,7 +387,7 @@ The array-based algorithm is equal to the recursive description.
     Array.size (countModelsStep I numVars i O) = O.size + 1 := by
   simp [countModelsStep]
 
-@[simp] theorem get_countModelsStep_of_lt (I : Array IteElt) (numVars : Nat) (O : Array Nat) 
+@[simp] theorem get_countModelsStep_of_lt (I : Array IteElt) (numVars : Nat) (O : Array Nat)
       (i j : Nat) (hi : i < O.size) :
     (countModelsStep I numVars j O)[i] = O[i] := by
   simp [countModelsStep]; rw [Array.get_push_of_lt O _ hi]
@@ -254,31 +401,31 @@ The array-based algorithm is equal to the recursive description.
         | Ite c t f  => (O[t] + O[f]) / 2 := by
   simp [countModelsStep]
 
-def countModelsRec (I : Array IteElt) (numVars : Nat) (n j : Nat) (init : Array Nat) : Array Nat := 
+def countModelsRec (I : Array IteElt) (numVars : Nat) (n j : Nat) (init : Array Nat) : Array Nat :=
   Std.Range.forIn.loop (m := Id) [:I.size]
     (fun i (O : Array Nat) => ForInStep.yield $ countModelsStep I numVars i O) n j init
 
 theorem countModels_eq_countModelsRec (I : Array IteElt) (numVars : Nat) :
   countModels I numVars = countModelsRec I numVars I.size 0 #[] := rfl
 
-theorem countModelsRecSucc (I : Array IteElt) (numVars : Nat) (n j : Nat) (init : Array Nat) : 
+theorem countModelsRecSucc (I : Array IteElt) (numVars : Nat) (n j : Nat) (init : Array Nat) :
     countModelsRec I numVars (n + 1) j init =
       if j ≥ Array.size I then init else
         countModelsRec I numVars n (j + 1) (countModelsStep I numVars j init) := by
   simp [countModelsRec]
 
 theorem countModelsRec_prop (I : Iteg) (numVars : Nat) : ∀ n j (init : Array Nat),
-  init.size = j → (∀ i, i < j → init[i] = I.count numVars i) → n + j ≤ I.val.size →  
+  init.size = j → (∀ i, i < j → init[i] = I.count numVars i) → n + j ≤ I.val.size →
     let O := countModelsRec I.val numVars n j init
     O.size = n + j ∧ ∀ i, i < n + j → O[i] = I.count numVars i
 | 0, j, init, h₁, h₂, _ => by
   simp [countModelsRec]
-  exact ⟨h₁, fun i hi => h₂ _ hi⟩ 
+  exact ⟨h₁, fun i hi => h₂ _ hi⟩
 | n+1, j, init, h₁, h₂, h₃ => by
   simp [countModelsRecSucc]
   let O := countModelsStep I.val numVars j init
-  have h₄ : Array.size O = j + 1 by simp [h₁]
-  have h₅ : ∀ i, i < j + 1 → O[i] = count I numVars i by
+  have h₄ : Array.size O = j + 1 := by simp [h₁]
+  have h₅ : ∀ i, i < j + 1 → O[i] = count I numVars i := by
     intros i hi
     cases Nat.le_iff_lt_or_eq.mp $ Nat.lt_succ_iff_le.mp hi with
       | inl h' =>
@@ -286,16 +433,16 @@ theorem countModelsRec_prop (I : Iteg) (numVars : Nat) : ∀ n j (init : Array N
         rw [h₁]; apply h'
       | inr h' =>
         rw [h', ←h₁, get_countModelsStep_size, count_eq, h₁]
-        cases ieq: I.val[j] with 
-          | Ite c t f => 
-            have bdd : IteEltBounded (Ite c t f) j by { rw ←ieq; apply I.property }
+        cases ieq: I.val[j] with
+          | Ite c t f =>
+            have bdd : IteEltBounded (Ite c t f) j := by { rw [←ieq]; apply I.property }
             simp [h₂ _ bdd.1, h₂ _ bdd.2]
           | _ => rfl
-  have h₆ : n + (j + 1) = n + 1 + j by rw [Nat.add_assoc, Nat.add_comm j]
-  have h₇ : n + (j + 1) ≤ I.val.size by rw [h₆]; exact h₃ 
+  have h₆ : n + (j + 1) = n + 1 + j := by rw [Nat.add_assoc, Nat.add_comm j]
+  have h₇ : n + (j + 1) ≤ I.val.size := by rw [h₆]; exact h₃
   let ih := countModelsRec_prop I numVars n (j+1) (countModelsStep I.val numVars j init) h₄ h₅ h₇
-  have h₇ : ¬ j ≥ I.val.size by
-    apply Nat.not_le_of_lt
+  have h₇ : ¬ j ≥ I.val.size := by
+    apply Nat.not_le_of_gt
     apply Nat.lt_of_lt_of_le _ h₃
     rw [Nat.add_comm (n + 1), ←Nat.add_assoc]
     apply Nat.lt_succ_of_le
@@ -305,7 +452,7 @@ theorem countModelsRec_prop (I : Iteg) (numVars : Nat) : ∀ n j (init : Array N
 
 theorem countModels_eq_count (I : Iteg) (numVars : Nat) {j} (hj : j < I.val.size) :
     (countModels I.val numVars)[j] = I.count numVars j :=
-  (countModelsRec_prop I numVars I.val.size 0 #[] Array.size_empty 
+  (countModelsRec_prop I numVars I.val.size 0 #[] Array.size_empty
     (fun _ hi => absurd hi (Nat.not_lt_zero _)) (Nat.le_refl _)).2 _ hj
 
 end Iteg
