lean4/ModelCount/ModelCount.lean
@@ -5,7 +5,7 @@ def defaultFile := "/home/avigad/projects/model-counting/benchmarks/parity/parit
 def main (args : List String) : IO Unit := do
   let p ← timeit "Time spent parsing:" (readIteg $ args.getD 0 defaultFile)
   match p with
-    | (numInputs, output, numIteElts, I) => do 
+    | (numInputs, output, numIteElts, I) => do
       let O ← timeit "Time spent counting:" (Iteg.countModels I numInputs)
       IO.println s!"Result: {O[output]}"
       IO.println s!"Number of ite elements: {numIteElts}"
